Weidenbach_Book/IsaSAT_Initialisation.thy
@@ -1865,7 +1865,7 @@ definition finalise_init_code :: \<open>opts \<Rightarrow> twl_st_wl_heur_init \
      let lcount = 0;
     RETURN (M', N', D', Q', W', ((ns, m, the fst_As, the lst_As, next_search), to_remove),
        clvls, cach, lbd, take 1(replicate 160 (Pos 0)), init_stats,
-        (fema, sema, ccount, 0, \<phi>, 0, replicate (length \<phi>) False, 0, replicate (length \<phi>) False, 10000, 0, 0), vdom, [], lcount, opts, [])
+        (fema, sema, ccount, 0, \<phi>, 0, replicate (length \<phi>) False, 0, replicate (length \<phi>) False, 10000, 1000, 1000), vdom, [], lcount, opts, [])
      })\<close>
 
 lemma isa_vmtf_init_nemptyD: \<open>((ak, al, am, an, bc), ao, bd)
